example.v
@@ -1,0 +1,208 @@
+From mathcomp Require Import ssreflect ssrnat eqtype ssrbool ssrfun seq.
+From mathcomp Require Import finmap choice finfun fintype.
+From coqspec Require Import int utilities substitution dev.
+
+Definition x1    : Var   :=  1.
+Definition x2    : Var   :=  2.
+Definition YES   : Val   := '3.
+Definition NO    : Val   := '4.
+Definition h1    : Var   :=  3.
+Definition h2    : Var   :=  4.
+Definition t1    : Var   :=  5.
+Definition t2    : Var   :=  6.
+Definition h1'   : Var   :=  7.
+Definition h2'   : Var   :=  8.
+Definition eqStr : FName :=  1.
+
+Notation "'If' c 'Then' t1 'Else' t2" := (COND c t1 t2) (at level 50).
+Notation "'Case' x 'Of' '|' h & t '-->' t1 '|' 'ATOM' '-->' t2" := 
+  (COND (CONS? x) (HT h t x t1) t2) (at level 100).
+Notation "x =? y" := (EQA? x y) (at level 10).
+Notation "a $ b"  := (CALL a b) (at level 10).
+
+Definition eq_str : Def := 
+  DEFINE eqStr [:: x1; x2] (
+    Case x1 Of 
+    | h1 & t1 --> 
+        Case x2 Of
+        |  h2 & t2 -->
+            If h1 =? h2 Then
+              eqStr $ [:: (t1 : Exp); (t2 : Exp)]
+            Else NO
+        |  ATOM --> NO
+    | ATOM --> 
+        If (CONS? x2) Then
+          NO
+        Else If x1 =? x2 Then
+          YES
+        Else NO
+  ).
+
+Arguments dev : simpl nomatch.
+Arguments caller : simpl never.
+
+Lemma example: 
+  specn 2 eq_str [:: CONS '3 '4] [:: eq_str] = 
+  DEFINE eqStr [:: x2] (
+    Case x2 Of 
+    | h1' & h2' --> 
+        If '3 =? h1' Then
+          If CONS? h2' Then NO
+          Else If '4 =? h2' Then YES
+          Else NO
+        Else NO
+    | ATOM --> NO).
+Proof.
+have H: ((fun=> id) @2` ([:: Exp_Arg t1; Exp_Arg t2], FVExp)) = [fset t1; t2].
+apply/fsetP=> x.
+apply/imfset2P; rewrite ?inE.
+case: (boolP (x == t1))=> [/eqP->|] /=.
+- exists t1=> //; exists t1=> /=; by rewrite ?inE.
+case: ifP=> [/eqP->|+/negbTE+[?+[?+E]]].
+- do? exists t2=> //; by rewrite ?inE.
+by rewrite ?inE E=> N1 N2 /orP[]/eqP-> /=; rewrite ?inE (N1, N2).
+
+rewrite /specn /devn /spec /= {1}/caller /=.
+move=> /=.
+suff->: (maxn
+      (maxn (maxvar (CALL 1 [:: Exp_Arg x1; Exp_Arg x2]))
+          (max_set (whole (mkEnv [:: x1; x2] [:: CONS ' (3) ' (4)], [::]))))
+      (maxvar
+          (If CONStest x1
+          Then HT h1 t1 x1
+                  (If CONStest x2
+                  Then HT h2 t2 x2
+                          (If ATOMtest h1 h2 Then CALL 1 [:: Exp_Arg t1; Exp_Arg t2] Else NO)
+                  Else NO)
+          Else (If CONStest x2 Then NO
+                Else (If ATOMtest x1 x2 Then YES Else NO))))) = 6.
+set f := caller [:: eq_str; eq_str] (dev id_call).
+rewrite /dev.
+suff->: dev_cntr (CONStest x1)
+(mkEnv [:: x1; x2]
+    [:: mkEnv [:: x1; x2] [:: CONS ' (3) ' (4)] x1;
+        mkEnv [:: x1; x2] [:: CONS ' (3) ' (4)] x2], [::]) = 
+CTRUE ([fsfun emsub with x1 |-> CONS '3 '4 ], [::]).
+rewrite /subst fsfun_with.
+suff->: (dev_cntr (CONStest x2)
+([fsfun emsub with h1 |-> (Exp_Arg ' (3)), t1 |-> (Exp_Arg ' (4)), x1 |-> CONS ' (3) ' (4)],
+[::])) = CBOTH (CONStest x2) ([fsfun emsub with h1 |->  Exp_Arg ' (3), t1 |->  Exp_Arg ' (4), x1 |-> CONS ' (3) ' (4)],
+[::]) ([fsfun emsub with h1 |-> Exp_Arg ' (3), t1 |-> Exp_Arg ' (4), x1 |-> CONS ' (3) ' (4)],
+[:: NCONS x2]).
+rewrite ?fsfun_withE emsubv.
+do 3? case: (boolP (_ == _))=> *; try slia.
+have->: dev_cntr (ATOMtest h1 h2)
+([fsfun emsub
+  with x2 |-> CONS (Exp_Arg (Arg_Var 7)) (Exp_Arg (Arg_Var 8)), h2 |-> (Exp_Arg (Arg_Var 7)), 
+        t2 |-> Exp_Arg (Arg_Var 8), h1 |-> Exp_Arg ' (3), t1 |-> Exp_Arg ' (4),
+        x1 |-> CONS ' (3) ' (4)], [::]) =
+        CBOTH (ATOMtest (Exp_Arg (Arg_Val ' (3))) (Exp_Arg (Arg_Var 7)))
+        (comp
+            [fsfun emsub
+            with x2 |-> CONS (Exp_Arg (Arg_Var 7)) (Exp_Arg (Arg_Var 8)),
+                  h2 |-> Exp_Arg (Arg_Var 7), t2 |-> Exp_Arg (Arg_Var 8),
+                  h1 |-> Exp_Arg (Arg_Val ' (3)), t1 |-> Exp_Arg (Arg_Val ' (4)),
+                  x1 |-> CONS (Exp_Arg (Arg_Val ' (3))) (Exp_Arg (Arg_Val ' (4)))]
+            [fsfun emsub with 7 |-> Exp_Arg (Arg_Val ' (3))], [::])
+        ([fsfun emsub
+          with x2 |-> CONS (Exp_Arg (Arg_Var 7)) (Exp_Arg (Arg_Var 8)),
+                h2 |-> Exp_Arg (Arg_Var 7), t2 |-> Exp_Arg (Arg_Var 8),
+                h1 |-> Exp_Arg (Arg_Val ' (3)), t1 |-> Exp_Arg (Arg_Val ' (4)),
+                x1 |-> CONS (Exp_Arg (Arg_Val ' (3))) (Exp_Arg (Arg_Val ' (4)))],
+        [:: (Arg_Var 7) ≠ (Arg_Val ' (3))]).
+rewrite /dev_cntr /subst /= ?fsfun_withE ?eq_refl.
+do 3? case: (boolP (_ == _))=> * //; try slia.
+rewrite /NO /id_call /= ?comp_var /= ?fsfun_withE ?eq_refl /= ?fsfun_withE emsubv.
+have-> //: (8 == 7) = false by slia.
+suff->:  (maxn 9
+(maxvar
+    (If CONStest (Arg_Var x1)
+    Then HT h1 t1 x1
+            (If CONStest (Arg_Var x2)
+            Then HT h2 t2 x2
+                    (If ATOMtest 
+                          (Exp_Arg (Arg_Var h1))
+                          (Exp_Arg (Arg_Var h2))
+                    Then CALL 1
+                            [::
+                            Exp_Arg (Arg_Var t1);
+                            Exp_Arg (Arg_Var t2)]
+                    Else RET (Exp_Arg (Arg_Val NO)))
+            Else RET (Exp_Arg (Arg_Val NO)))
+    Else (If CONStest (Arg_Var x2)
+          Then RET (Exp_Arg (Arg_Val NO))
+          Else (If ATOMtest (Exp_Arg (Arg_Var x1))
+                      (Exp_Arg (Arg_Var x2))
+                Then RET (Exp_Arg (Arg_Val YES))
+                Else RET (Exp_Arg (Arg_Val NO))))))) = 9.
+
+rewrite /dev. 
+
+have->: dev_cntr (CONStest x1)
+(mkEnv [:: x1; x2] [:: Exp_Arg ' (4); Exp_Arg (Arg_Var 8)], [::]) =
+CFALSE
+([fsfun emsub
+  with x1 |-> Exp_Arg (Arg_Val ' (4)), x2 |-> Exp_Arg (Arg_Var 8)], [::]).
+- rewrite /dev_cntr /= /mkEnv /= fsfun_with //.
+have->: dev_cntr (CONStest x2)
+([fsfun emsub with x1 |-> Exp_Arg ' (4), x2 |-> Exp_Arg (Arg_Var 8)], [::]) = 
+CBOTH (CONStest (Arg_Var 8))
+(comp
+    [fsfun emsub
+    with x1 |-> Exp_Arg (Arg_Val ' (4)), x2 |-> Exp_Arg (Arg_Var 8)] emsub,
+[::])
+([fsfun emsub
+  with x1 |-> Exp_Arg (Arg_Val ' (4)), x2 |-> Exp_Arg (Arg_Var 8)],
+[:: NCONS (Arg_Var 8)]).
+- rewrite /dev_cntr /= fsfun_withE.
+  case: (boolP (_ == _)); try slia.
+  rewrite fsfun_with //.
+have-> //=: dev_cntr (ATOMtest x1 x2)
+([fsfun emsub with x1 |-> (Exp_Arg '(4)), x2 |->  Exp_Arg (Arg_Var 8)],
+[:: NCONS (Arg_Var 8)]) = CBOTH (ATOMtest (Exp_Arg (Arg_Val ' (4))) (Exp_Arg (Arg_Var 8)))
+(comp
+    [fsfun emsub
+    with x1 |-> Exp_Arg (Arg_Val ' (4)), x2 |-> Exp_Arg (Arg_Var 8)]
+    [fsfun emsub with 8 |-> Exp_Arg (Arg_Val ' (4))],
+[:: NCONS (Arg_Var 8)])
+([fsfun emsub
+  with x1 |-> Exp_Arg (Arg_Val ' (4)), x2 |-> Exp_Arg (Arg_Var 8)],
+[:: (Arg_Var 8) ≠ (Arg_Val ' (4)); NCONS (Arg_Var 8)]).
+- rewrite /dev_cntr /= fsfun_with fsfun_withE.
+  case: (boolP (_ == _)); try slia.
+  rewrite fsfun_with //=.
+
+rewrite /maxvar ?max_setU /= ?max_set1 H.
+by rewrite max_setU /max_set ?enum_fsetE /= ?enum_fset1 /=.
+rewrite /dev_cntr /= ?fsfun_withE emsubv.
+
+do 3? case: (boolP (_ == _))=> * //; try slia.
+by congr CBOTH; congr (_,_); rewrite compe0.
+
+rewrite /dev_cntr /= /mkEnv /= ?fsfun_with ?fsfun_withE emsubv.
+have->: (x2 == x1) = false by slia.
+
+congr CTRUE; congr (_,_); apply/fsfunP=> ?.
+by rewrite ?fsfun_withE emsubv; (do ? case: ifP=> //) => /eqP->.
+rewrite /maxvar.
+
+rewrite /VTree /= ?max_setU ?H ?max_set0 /= ?max_setU.
+have->: ((fun=> id) @2` ([:: Exp_Arg x1; Exp_Arg x2], FVExp)) = [fset x1; x2].
+apply/fsetP=> x.
+apply/imfset2P; rewrite ?inE.
+case: (boolP (x == x1))=> [/eqP->|] /=.
+- exists x1=> //; exists x1=> /=; by rewrite ?inE.
+case: ifP=> [/eqP->|+/negbTE+[?+[?+E]]].
+- do? exists x2=> //; by rewrite ?inE.
+by rewrite ?inE E=> N1 N2 /orP[]/eqP-> /=; rewrite ?inE (N1, N2).
+rewrite max_setU ?max_set1 /whole_rs.
+have->: (fun=> id) @2` ([::], FVRestr) = fset0.
+apply/fsetP=> ?; apply/imfset2P; rewrite ?inE=> [[/= ?]].
+by rewrite ?inE.
+rewrite max_set0 /mkEnv /=.
+have->: (whole_env [fsfun emsub with x1 |-> CONS ' (3) ' (4)]) = fset0.
+apply/fsetP=> ?; apply/imfset2P; rewrite ?inE=> [[/= ?]].
+rewrite finsupp_with /= ?inE orbF=> /eqP-> [?].
+by rewrite fsfun_with /= ?inE.
+by rewrite max_set0.
+Qed.
